size-classes: remove admits 7/7: done!
lets check extraction and merge

src/Slabs.fst
@@ -738,11 +738,26 @@ let alloc_metadata_aux
   return b
 #pop-options
 
+#push-options "--fuel 0 --ifuel 0"
 let empty_md_is_properly_zeroed
   (size_class: sc)
   : Lemma
   (slab_vprop_aux2 size_class (Seq.create 4 0UL))
-  = admit ()
+  =
+  let zero_to_vec_lemma2 (i:nat{i < 64})
+    : Lemma
+    (FU.nth (FU.zero 64) i = false)
+    =
+    FU.zero_to_vec_lemma #64 i in
+  let s0 = Seq.create 4 0UL in
+  let bm = Bitmap4.array_to_bv2 #4 s0 in
+  let bound2 = bound2_gen (nb_slots size_class) (G.hide size_class) in
+  assert (U64.v (Seq.index s0 0) == FU.zero 64);
+  array_to_bv_slice #4 s0 0;
+  Classical.forall_intro (zero_to_vec_lemma2);
+  Seq.lemma_eq_intro (Seq.slice bm 0 64) (Seq.create 64 false);
+  zf_b_slice (Seq.slice bm 0 64) 0 (64 - U32.v bound2)
+#pop-options
 
 #push-options "--z3rlimit 100 --compat_pre_typed_indexed_effects"
 let alloc_metadata_aux2
